\input{body/G_0.tex}

\section{Non-triviality and distinctness of the four generators}
\label{section:identityProofs}

\noindent{}Recall that
\begin{align*}
G_n=\langle a,\; b,\; c,\; d \mid{} &(a^{-1}b)^{10n}d^{-1}a^{2},\; b^{-2}c(b^{-1}a)^{10n},\\
&(d^{-1}c)^{10n+3}c^{-1}bc^{-2},\; d^{2}a^{-1}d(c^{-1}d)^{10n+3} \rangle
\end{align*}
for integers $n\geq{}0$.

\vspace{10pt}

\begin{proposition}
The four generators of $G_n$ are all distinct and non-trivial.
\label{proposition:non-trivial}
\end{proposition}
\begin{proof}
Greene and Watson \cite[Section 4.2]{GreeneWatson} show that the abelianization of $G_n$ provides a homomorphism:
\begin{align*}
\phi:G_n\rightarrow \mathbb{Z}_{25}
\end{align*}
with $\phi(a)=13$, $\phi(b)=3$, $\phi(c)=6$, and $\phi(d)=1$. Because each of the generators maps to a distinct, non-identity element of $\mathbb{Z}_{25}$, it follows that the four generators are distinct and nontrivial.
\end{proof}

\begin{corollary}
Both $bc^{-3}$ and $ad^{-3}$ are non-trivial.
\label{corollary:non-trivial2}
\end{corollary}
\begin{proof}
By the third group relation, we have:
\begin{align*}
(d^{-1}c)^{10n+3}c^{-1}bc^{-2}&=1\\
\Rightarrow{}(cd^{-1})^{10n+3}bc^{-3}&=1\\
\Rightarrow{}bc^{-3}&=(dc^{-1})^{10n+3}.
\end{align*}
By Proposition~\ref{proposition:non-trivial}, $dc^{-1}\ne1$, therefore $bc^{-3}\ne1$.\\

\noindent{}By the fourth group relation, we have:
\begin{align*}
(d^{-1}c)^{10n+3}d^{-1}ad^{-2}&=1\\
\Rightarrow{}(cd^{-1})^{10n+3}ad^{-3}&=1\\
\Rightarrow{}ad^{-3}&=(dc^{-1})^{10n+3}.
\end{align*}
By Proposition~\ref{proposition:non-trivial}, $dc^{-1}\ne1$, therefore $ad^{-3}\ne1$.
\end{proof}

\noindent{}We will assume $G_n$ is left-orderable and then reach a contradiction. By Fact~\ref{fact:WLOG}, we can assume without loss of generality that $b^{-1}a\geq1$. Because of Proposition~\ref{proposition:non-trivial}, we can assume (without loss of generality) that $b^{-1}a>1$.\\

\noindent{}With four (non-trivial) group generators there are 16 possible cases for the signs of each of the generators that must be considered (see Table~\ref{table:casesAll}). We will disprove each of these cases.



\begin{table}[ht]
\begin{center}
\begin{tabular}{l | l | l | l | l}
Case\hspace{10 pt} & $a$\hspace{10 pt} & $b$\hspace{10 pt} & $c$\hspace{10 pt} & $d$\hspace{10 pt} \\\hline\hline
1 & $+$ & $+$ & $+$ & $+$ \\\hline
2 & $+$ & $+$ & $+$ & $-$ \\\hline
3 & $+$ & $+$ & $-$ & $+$ \\\hline
4 & $+$ & $+$ & $-$ & $-$ \\\hline
5 & $+$ & $-$ & $+$ & $+$ \\\hline
6 & $+$ & $-$ & $+$ & $-$ \\\hline
7 & $+$ & $-$ & $-$ & $+$ \\\hline
8 & $+$ & $-$ & $-$ & $-$ \\\hline
9 & $-$ & $+$ & $+$ & $+$ \\\hline
10 & $-$ & $+$ & $+$ & $-$ \\\hline
11 & $-$ & $+$ & $-$ & $+$ \\\hline
12 & $-$ & $+$ & $-$ & $-$ \\\hline
13 & $-$ & $-$ & $+$ & $+$ \\\hline
14 & $-$ & $-$ & $+$ & $-$ \\\hline
15 & $-$ & $-$ & $-$ & $+$ \\\hline
16 & $-$ & $-$ & $-$ & $-$ 
\end{tabular}
\end{center}
\caption{The 16 possible cases with 4 generators}
\label{table:casesAll}
\end{table}

\section{General Lemmas}
\label{section:generalLemmas}

\noindent{}First we prove some lemmas that will be used later. These lemmas are true for all cases listed in Table~\ref{table:casesAll}.

\begin{lemma} In $G_n$, $d^{-1}a^{2}=c^{-1}b^{2}$.
\label{lemma:eq5}
\end{lemma}
\begin{proof} The first group relation for $G_n$ can be rearranged as follows:
\begin{align}
(a^{-1}b)^{10n}d^{-1}a^{2}&=1\nonumber{}\\
\Rightarrow{}(b^{-1}a)^{10n}&=d^{-1}a^{2},\label{eq1:2}
\end{align}
and the second group relation can be rearranged as follows:
\begin{align}
b^{-2}c(b^{-1}a)^{10n}&=1\nonumber{}\\
\Rightarrow{}(b^{-1}a)^{10n}&=c^{-1}b^{2}.\label{eq2:2}
\end{align}
This shows that:
\begin{align*}
d^{-1}a^{2}&=c^{-1}b^{2}.\qedhere
\end{align*}
\end{proof}

\begin{corollary} In $G_n$, $a^{2}b^{-2}=dc^{-1}$.
\label{corollary:eq6}
\end{corollary}
\begin{proof}By Lemma~\ref{lemma:eq5} we know:
\begin{align*}
d^{-1}a^{2}&=c^{-1}b^{2}\\
\Rightarrow{}a^{2}b^{-2}&=dc^{-1}.\qedhere
\end{align*}
\end{proof}

\begin{lemma} In $G_n$, $d^{2}a^{-1}d=c^{2}b^{-1}c$.
\label{lemma:eq7}
\end{lemma}
\begin{proof}
The third group relation for $G_n$ can be rearranged as follows:
\begin{align*}
(d^{-1}c)^{10n+3}c^{-1}bc^{-2}&=1\\
\Rightarrow{}(d^{-1}c)^{10n+3}&=c^{2}b^{-1}c,
\end{align*}
and the fourth group relation can be rearranged as follows:
\begin{align*}
d^{2}a^{-1}d(c^{-1}d)^{10n+3}&=1\\
\Rightarrow{}(d^{-1}c)^{10n+3}&=d^{2}a^{-1}d.
\end{align*}
Showing that:
\begin{align}
\label{eq7}d^{2}a^{-1}d&=c^{2}b^{-1}c.
\end{align}
\end{proof}

\begin{lemma} In $G_n$, $d^{2}a=c^{2}b$.
\label{lemma:eq8}
\end{lemma}
\begin{proof}
Starting from Lemma~\ref{lemma:eq5}, we have:
\begin{align}
d^{-1}a^{2}&=c^{-1}b^{2}\nonumber{}\\
\Rightarrow{}c&=b^{2}a^{-2}d.\label{eq5:2}
\end{align}
Using (\ref{eq5:2}), we can substitute for the right-most $c$ in (\ref{eq7}). We find:
\begin{align*}
d^{2}a^{-1}d&=c^{2}b^{-1}b^{2}a^{-2}d\\
\Rightarrow{}d^{2}a^{-1}d&=c^{2}ba^{-2}d\\
\Rightarrow{}d^{2}a&=c^{2}b.\qedhere
\end{align*}
\end{proof}

\begin{lemma} In $G_n$, $ad^{-1}a=bc^{-1}b$.
\label{lemma:eq16}
\end{lemma}
\begin{proof} By the first group relation, we have:
\begin{align}
(a^{-1}b)^{10n}d^{-1}a^{2}&=1\nonumber{}\\
\Rightarrow{}(a^{-1})(ba^{-1})^{10n}ad^{-1}a^{2}&=1\nonumber{}\\
\Rightarrow{}(ba^{-1})^{10n}ad^{-1}a&=1.\label{eq1:3}
\end{align}
By the second group relation, we have:
\begin{align}
b^{-2}c(b^{-1}a)^{10n}&=1\nonumber{}\\
\Rightarrow{} b^{-2}cb^{-1}(ab^{-1})^{10n}b&=1\nonumber{}\\
\Rightarrow{}b^{-1}cb^{-1}(ab^{-1})^{10n}&=1\nonumber{}\\
\Rightarrow{}b^{-1}cb^{-1}&=(ba^{-1})^{10n}.\label{eq2:3}
\end{align}
Substituting (\ref{eq2:3}) into (\ref{eq1:3}), we see:
\begin{align*}
b^{-1}cb^{-1}ad^{-1}a&=1\\
\Rightarrow{}ad^{-1}a&=bc^{-1}b.\qedhere
\end{align*}
\end{proof}

\begin{lemma} In $G_n$, $c^{-3}d^{3}=b^{-1}a$.
\label{lemma:eq9}
\end{lemma}
\begin{proof} By the third group relation, we have:
\begin{align}
(d^{-1}c)^{10n+3}c^{-1}bc^{-2}&=1\nonumber{}\\
\Rightarrow{}c^{-1}(cd^{-1})^{10n+3}bc^{-2}&=1\nonumber{}\\
\Rightarrow{}(cd^{-1})^{10n+3}bc^{-3}&=1.\label{eq3:33}
\end{align}
By the fourth group relation, we have:
\begin{align}
d^{2}a^{-1}d(c^{-1}d)^{10n+3}&=1\nonumber{}\\
\Rightarrow{}d^{2}a^{-1}(dc^{-1})^{10n+3}d&=1\nonumber{}\\
\Rightarrow{}d^{3}a^{-1}(dc^{-1})^{10n+3}&=1\nonumber{}\\
\Rightarrow{}d^{3}a^{-1}&=(cd^{-1})^{10n+3}.\label{eq4:33}
\end{align}
Substituting (\ref{eq4:33}) into (\ref{eq3:33}), we see:
\begin{align*}
d^{3}a^{-1}bc^{-3}&=1\\
\Rightarrow{}c^{-3}d^{3}&=b^{-1}a.\qedhere
\end{align*}
\end{proof}

\begin{corollary} If $G_n$ is left-orderable, then $c^{-3}d^{3}>1$.
\label{corollary:inEq5}
\end{corollary}
\begin{proof}This is an immediate consequence of Lemma~\ref{lemma:eq9} and the general assumption that $b^{-1}a>1$.
\end{proof}

\begin{lemma} If $G_n$ is left-orderable, then $d^{-1}a^{2}>1$.
\label{lemma:inEq3}
\end{lemma}
\begin{proof}By (\ref{eq1:2}) we have:
\begin{align*}
(b^{-1}a)^{10n}&=d^{-1}a^{2},
\end{align*}
and since we are assuming $b^{-1}a>1$, this shows that $d^{-1}a^{2}>1$.
\end{proof}

\begin{lemma} If $G_n$ is left-orderable, then $d^{-2}c^{2}b^{-1}cd^{-1}b<1$.
\label{lemma:inEq7}
\end{lemma}
\begin{proof} By  Lemma~\ref{lemma:eq7} we have:
\begin{align}
d^{2}a^{-1}d&=c^{2}b^{-1}c\nonumber{}\\
\Rightarrow{}d^{2}&=c^{2}b^{-1}cd^{-1}a.\label{eq7:2}
\end{align}
By rearranging the result of Lemma~\ref{lemma:eq9} we have:
\begin{align*}
c^{3}=d^{3}a^{-1}b=d(c^{2}b^{-1}cd^{-1}a)a^{-1}b.
\end{align*}
Note that the last equality follows by substituting for $d^{2}$ using (\ref{eq7:2}). This expression can be rearranged to give:
\begin{align}
d&=c^{3}b^{-1}dc^{-1}bc^{-2}\nonumber{}\\
\Rightarrow{}c^{-1}d&=c^2b^{-1}dc^{-1}bc^{-2}.\label{eq13}
\end{align}
Now (\ref{eq13}) can be rearranged to yield:
\begin{align}
d^{-1}c^3b^{-1}dc^{-1}bc^{-2}&=1\nonumber{}\\
\Rightarrow{}(d^{-3}c^3)(b^{-1}dc^{-1}bc^{-2}d^{2})&=1.\label{lemma:inEq7:contradiction}
\end{align}
By Corollary~\ref{corollary:inEq5}, $d^{-3}c^3<1$, therefore (\ref{lemma:inEq7:contradiction}) shows that:
\begin{align*}
b^{-1}dc^{-1}bc^{-2}d^{2}&>1\\
\Rightarrow{}d^{-2}c^{2}b^{-1}cd^{-1}b&<1.\qedhere
\end{align*}
\end{proof}

\begin{lemma} If $G_n$ is left-orderable, then $c^{-1}ba^{-1}d>1$.
\label{lemma:inEq:CbAd}
\end{lemma}
\begin{proof} By Lemma~\ref{lemma:eq16}, we have:
\begin{align}
a^{-1}da^{-1}bc^{-1}b&= 1\nonumber{}\\
\Rightarrow{}c^{-1}ba^{-1}da^{-1}b &=1\nonumber{}\\
\Rightarrow{}(b^{-1}a)(d^{-1}ab^{-1}c) &= 1.\label{lemma:inEq:CbAd:contradiction}
\end{align}
We know $b^{-1}a>1$, so (\ref{lemma:inEq:CbAd:contradiction}) shows that:
\begin{align*}
d^{-1}ab^{-1}c&<1\\
\Rightarrow{}c^{-1}ba^{-1}d&>1.\qedhere
\end{align*}
\end{proof}

\begin{lemma} If $G_n$ is left-orderable, then $b<1$ implies $c<1$.
\label{genImp1}
\end{lemma}
\begin{proof}By Lemma~\ref{lemma:inEq3}, $d^{-1}a^{2}>1$, and hence $a^{-2}d<1$. By Lemma~\ref{lemma:eq5}, we have:
\begin{align*}
d^{-1}a^{2}&=c^{-1}b^{2}\\
\Rightarrow{}c&=b^{2}a^{-2}d,
\end{align*}
and it is now easy to see that:
\begin{align*}
b<1\Rightarrow{}b^{2}<1\Rightarrow{}b^{2}a^{-2}d&<1\Rightarrow{}c<1.\qedhere
\end{align*}
\end{proof}

\input{body/cases2-15}

%end{case8}
%begin{case1}

\input{body/case_1}

\input{body/case_16}

\noindent{}With Proposition~\ref{proposition:case16.B}, we have eliminated the final sub-case of Case 16. We have therefore shown that $G_n$ is not left-orderable.


